haetae-topdown-easycrypt/post-freeze/VerifyUnpackV3NttBound17PostFreeze.ec
@@ -1,0 +1,815 @@
+require import AllCore IntDiv List.
+
+from Jasmin require import JModel_x86.
+
+import SLH64.
+
+require import BArray8192 Array256 Fq GFq Rq.
+require import Hpoly_loop VerifyUnpackMode2Target.
+require import NTT_Fq NTTFullSpec NTTFullAlgebra NTTRowProductSpec.
+require import RefJasminNTTLoop TargetNTTRefinement
+               TargetKeygenM23WideNTT TargetKeygenM23WideSupport
+               KeygenM23ArithmeticSpec KeygenM23MatrixSpec
+               VerifyUnpackV3NttPostFreeze.
+
+theory VerifyUnpackV3NttBound17PostFreeze.
+
+module Verify = VerifyUnpackMode2Target.M.
+module Parent = TargetKeygenM23WideSupport.Parent.
+module Wide = TargetKeygenM23WideNTT.WideSpec.
+module Target = TargetNTTRefinement.Target.
+
+import TargetKeygenM23WideSupport.
+import RefJasminNTT.
+
+op verify_unpack_ntt_polys : int = 2.
+op verify_unpack_ntt_words : int =
+  verify_unpack_ntt_polys * KeygenM23MatrixSpec.poly_words_i.
+
+op verify_unpack_ntt_input_repr_bound17
+    (s : BArray8192.t) (p0 p1 : Rq.poly) : bool =
+  KeygenM23ArithmeticSpec.wide_slice_repr_bound s 0 p0 17 /\
+  KeygenM23ArithmeticSpec.wide_slice_repr_bound
+    s KeygenM23MatrixSpec.poly_words_i p1 17.
+
+op verify_unpack_ntt_repr_bound25
+    (s : BArray8192.t) (p0 p1 : Rq.poly) : bool =
+  KeygenM23ArithmeticSpec.wide_slice_repr_bound
+    s 0 (NTTFullSpec.full_ntt p0) 25 /\
+  KeygenM23ArithmeticSpec.wide_slice_repr_bound
+    s KeygenM23MatrixSpec.poly_words_i
+    (NTTFullSpec.full_ntt p1) 25.
+
+op fwd_stage_bound17 (len : int) : int =
+  RefJasminNTT.fwd_stage_bound len + 1.
+
+lemma fwd_stage_bound17_range len :
+  RefJasminNTT.fwd_len_ok len =>
+  0 <= fwd_stage_bound17 len <= 25.
+proof.
+move=> hlen.
+have hrange := RefJasminNTT.fwd_stage_bound_range len hlen.
+rewrite /fwd_stage_bound17.
+smt().
+qed.
+
+lemma fwd_stage_bound17_ge16 len :
+  RefJasminNTT.fwd_len_ok len =>
+  16 <= fwd_stage_bound17 len.
+proof.
+move=> hlen.
+have hrange := fwd_stage_bound17_range len hlen.
+smt().
+qed.
+
+lemma fwd_stage_bound17_lt31 len :
+  RefJasminNTT.fwd_len_ok len =>
+  fwd_stage_bound17 len < 31.
+proof.
+move=> hlen.
+have hrange := fwd_stage_bound17_range len hlen.
+smt().
+qed.
+
+lemma fqmul_product_bound_16_25 a b :
+  Fq.bw32 a 16 =>
+  Fq.bw32 b 25 =>
+  - Fq.SignedReductions.R %/ 2 * Fq.q <=
+    W32.to_sint a * W32.to_sint b <
+    Fq.SignedReductions.R %/ 2 * Fq.q.
+proof.
+rewrite /Fq.bw32 /Fq.SignedReductions.R /Fq.q /=.
+smt().
+qed.
+
+lemma fwd_stage_bound17_next len :
+  RefJasminNTT.fwd_len_ok len =>
+  0 < len =>
+  fwd_stage_bound17 (len %/ 2) = fwd_stage_bound17 len + 1.
+proof.
+move=> hlen hpos.
+rewrite /fwd_stage_bound17.
+have hnext := RefJasminNTT.fwd_stage_next len hlen hpos.
+smt().
+qed.
+
+lemma forward_twiddle_product_bound_from_inner17
+  rp len start j zc :
+  barray256_bound_by rp
+    (fwd_inner_bound (fwd_stage_bound17 len) len start j) =>
+  fwd_len_ok len =>
+  0 < len =>
+  start <= j < start + len =>
+  0 <= j + len < 256 =>
+  1 <= zc < 256 =>
+  - Fq.SignedReductions.R %/ 2 * Fq.q <=
+    W32.to_sint (BArray1024.get32 Hpoly_loop.jzetas zc) *
+    W32.to_sint (BArray1024.get32 rp (j + len)) <
+    Fq.SignedReductions.R %/ 2 * Fq.q.
+proof.
+move=> hbd hlenok hlen hjrange hjlen hzc.
+have hzbw := jzetas_bound16 zc hzc.
+have [_ [hcurjl _]] :=
+  fwd_inner_current (fwd_stage_bound17 len) len start j _ hlen hjrange.
++ have hrange := fwd_stage_bound17_range len hlenok.
+  smt().
+have hraw :
+  Fq.bw32 (BArray1024.get32 rp (j + len)) (fwd_stage_bound17 len).
++ have hjlmem : j + len \in range 0 256 by rewrite mem_range; smt().
+  have := hbd (j + len) hjlmem.
+  by rewrite hcurjl.
+have hstage := fwd_stage_bound17_range len hlenok.
+have hbw25 :
+  Fq.bw32 (BArray1024.get32 rp (j + len)) 25.
++ exact (NTT_Fq.bw32_weaken (BArray1024.get32 rp (j + len))
+           (fwd_stage_bound17 len) 25 hstage hraw).
+exact (fqmul_product_bound_16_25
+  (BArray1024.get32 Hpoly_loop.jzetas zc)
+  (BArray1024.get32 rp (j + len)) hzbw hbw25).
+qed.
+
+equiv poly_ntt_core_ref17 :
+  Hpoly_loop.M._poly_ntt ~ NTT_Fq.NTT.ntt :
+  NTT_Fq.poly_repr_bound rp{1} r{2} 17 /\
+  zetas{2} = NTT_Fq.zetas
+  ==> NTT_Fq.poly_repr_bound res{1} res{2} 25.
+proof.
+proc.
+wp.
+while (
+  NTT_Fq.poly_repr rp{1} r{2} /\
+  barray256_bound_by rp{1}
+    (const_bound (fwd_stage_bound17 len{1})) /\
+  zetasp{1} = Hpoly_loop.jzetas /\
+  zetas{2} = NTT_Fq.zetas /\
+  zetasctr{1} = zetasctr{2} /\
+  len{1} = len{2} /\
+  fwd_len_ok len{1} /\
+  zetasctr{1} = fwd_zbase len{1}
+).
++ wp.
+  while (
+    NTT_Fq.poly_repr rp{1} r{2} /\
+    barray256_bound_by rp{1}
+      (fwd_middle_bound
+        (fwd_stage_bound17 len{1}) start{1}) /\
+    zetasp{1} = Hpoly_loop.jzetas /\
+    zetas{2} = NTT_Fq.zetas /\
+    zetasctr{1} = zetasctr{2} /\
+    len{1} = len{2} /\
+    fwd_len_ok len{1} /\
+    0 < len{1} /\
+    start{1} = start{2} /\
+    0 <= start{1} <= 256 /\
+    start{1} =
+      2 * len{1} *
+        (zetasctr{1} - fwd_zbase len{1})
+  ).
+  + wp.
+    while (
+      NTT_Fq.poly_repr rp{1} r{2} /\
+      barray256_bound_by rp{1}
+        (fwd_inner_bound
+          (fwd_stage_bound17 len{1})
+          len{1} start{1} j{1}) /\
+      zetasp{1} = Hpoly_loop.jzetas /\
+      zetas{2} = NTT_Fq.zetas /\
+      zetasctr{1} = zetasctr{2} /\
+      len{1} = len{2} /\
+      fwd_len_ok len{1} /\
+      0 < len{1} /\
+      start{1} = start{2} /\
+      0 <= start{1} < 256 /\
+      start{1} + 2 * len{1} <= 256 /\
+      start{1} =
+        2 * len{1} *
+        (zetasctr{1} - 1 - fwd_zbase len{1}) /\
+      1 <= zetasctr{1} < 256 /\
+      zeta_0{1} = BArray1024.get32 Hpoly_loop.jzetas zetasctr{1} /\
+      zeta_{2} = NTT_Fq.zetas.[zetasctr{2}] /\
+      j{1} = j{2} /\
+      cmp{1} = start{1} + len{1} /\
+      start{1} <= j{1} <= start{1} + len{1}
+    ).
+    + wp.
+      sp.
+      ecall{1} (forward_twiddle_product_bound_call_ph
+        rp{1} r{2} zetasctr{2} j{2} len{2} zeta_0{1} coeff{1}).
+      wp.
+      skip.
+      move=> &1 &2 /=.
+      move=> [hs [hoff [hcoeff [hinv hguards]]]].
+      move: hinv => [hrepr hinv].
+      move: hinv => [hbd hinv].
+      move: hinv => [hzetasp hinv].
+      move: hinv => [hzetas hinv].
+      move: hinv => [hzc_eq hinv].
+      move: hinv => [hlen_eq hinv].
+      move: hinv => [hlenok hinv].
+      move: hinv => [hlen hinv].
+      move: hinv => [hstart_eq hinv].
+      move: hinv => [hstart_rng hinv].
+      move: hinv => [hblock hinv].
+      move: hinv => [hzctr hinv].
+      move: hinv => [hzcrng hinv].
+      move: hinv => [hzeta0 hinv].
+      move: hinv => [hzeta hinv].
+      move: hinv => [hj_eq [hcmp hjrng]].
+      move: hstart_rng => [hstart0 hstartlt].
+      move: hzcrng => [hzc_lo hzc_hi].
+      move: hjrng => [hj_ge hj_le].
+      move: hguards => [hj_guard1 hj_guard2].
+      split.
+      + split; first exact hrepr.
+        split; first by smt().
+        split; first by smt().
+        split.
+        + by rewrite hzeta0 hzc_eq.
+        split.
+        + by rewrite hcoeff hoff hj_eq hlen_eq.
+        split.
+        + rewrite hzeta0 hcoeff hoff.
+          have hprod :=
+            forward_twiddle_product_bound_from_inner17
+              rp{1} len{1} start{1} j{1} zetasctr{1}
+              hbd hlenok hlen _ _ _.
+          + by smt().
+          + by smt().
+          + by smt().
+          move: hprod.
+          by rewrite /Hpoly_loop.jzetas.
+        move=> _.
+        rewrite hzeta0 hcoeff hoff.
+        have hprod :=
+          forward_twiddle_product_bound_from_inner17
+            rp{1} len{1} start{1} j{1} zetasctr{1}
+            hbd hlenok hlen _ _ _.
+        + by smt().
+        + by smt().
+        + by smt().
+        move: hprod.
+        by rewrite /Hpoly_loop.jzetas.
+      move=> _ result [ht hbwt].
+      have hstep :=
+        forward_butterfly_step_bound_by
+          rp{1} r{2} j{1} len{1} start{1} s{1} result
+          (fwd_stage_bound17 len{1})
+          hrepr hbd _ hlen _ _ _ hs _ _ hbwt.
+      + by smt().
+      + by smt().
+      + by smt().
+      + by smt().
+      + exact (fwd_stage_bound17_ge16 len{1} hlenok).
+      + have hrange := fwd_stage_bound17_range len{1} hlenok.
+        smt().
+      move: hstep.
+      rewrite ht -hzeta hj_eq hlen_eq.
+      move=> [hpoly hbound].
+      rewrite hoff hj_eq hlen_eq.
+      split.
+      + split; first exact hpoly.
+        split; first exact hbound.
+        by smt().
+      by smt().
+    wp.
+    skip.
+    move=> &1 &2 /=.
+    move=> [hm hguards].
+    move: hm => [hrepr hm].
+    move: hm => [hbd hm].
+    move: hm => [hzetasp hm].
+    move: hm => [hzetas hm].
+    move: hm => [hzc_eq hm].
+    move: hm => [hlen_eq hm].
+    move: hm => [hlenok hm].
+    move: hm => [hlen hm].
+    move: hm => [hstart_eq hm].
+    move: hm => [hstart_rng hzctr].
+    move: hguards => [hstart_guard1 hstart_guard2].
+    move: hstart_rng => [hstart_ge hstart_le].
+    have hstart_lt : 0 <= start{1} < 256 by smt().
+    have hblock :=
+      fwd_block_end_bound len{1} start{1} zetasctr{1}
+        hlenok hlen hstart_lt hzctr.
+    have hzcr :=
+      fwd_read_range len{1} start{1} zetasctr{1}
+        hlenok hlen hstart_lt hzctr.
+    split.
+    + split.
+      + split; first exact hrepr.
+        split.
+        + move=> i hi.
+          rewrite -fwd_middle_to_inner.
+          exact (hbd i hi).
+        split; first exact hzetasp.
+        split; first exact hzetas.
+        split; first by smt().
+        split; first exact hlen_eq.
+        split; first exact hlenok.
+        split; first exact hlen.
+        split; first exact hstart_eq.
+        split; first exact hstart_lt.
+        split; first exact hblock.
+        split; first by smt().
+        split; first exact hzcr.
+        split; first by rewrite hzetasp.
+        split; first by rewrite hzetas.
+        split; first exact hstart_eq.
+        by smt().
+      by smt().
+    move=> jL rpL jR rR hnotL hnotR hinv.
+    move: hinv => [hreprL hinv].
+    move: hinv => [hbdL hinv].
+    move: hinv => [hzetaspL hinv].
+    move: hinv => [hzetasL hinv].
+    move: hinv => [hzcL hinv].
+    move: hinv => [hlenL_eq hinv].
+    move: hinv => [hlenL_ok hinv].
+    move: hinv => [hlenL hinv].
+    move: hinv => [hstartL_eq0 hinv].
+    move: hinv => [hstartL_rng hinv].
+    move: hinv => [hblockL hinv].
+    move: hinv => [hzctrL hinv].
+    move: hinv => [hzcrL hinv].
+    move: hinv => [hzeta0L hinv].
+    move: hinv => [hzetaL hinv].
+    move: hinv => [hj_eqL [hcmpL hjrngL]].
+    move: hstartL_rng => [hstartL_ge hstartL_lt].
+    have hjL_ge : start{1} <= jL by smt().
+    have hjL_le : jL <= start{1} + len{1} by smt().
+    have hj_end : jL = start{1} + len{1} by smt().
+    have hstart_new : jL + len{1} = start{1} + 2 * len{1} by smt().
+    have hbdmid :
+      barray256_bound_by rpL
+        (fwd_middle_bound
+          (fwd_stage_bound17 len{1}) (jL + len{1})).
+    + move=> i hi.
+      have htmp := hbdL i hi.
+      have heq :=
+        fwd_inner_exit_to_middle
+          (fwd_stage_bound17 len{1}) len{1} start{1} i
+          hstartL_ge hlenL.
+      rewrite hstart_new.
+      move: htmp.
+      by rewrite hj_end heq.
+    split.
+    + split; first exact hreprL.
+      split; first exact hbdmid.
+      split; first exact hzetaspL.
+      split; first exact hzetasL.
+      split; first exact hzcL.
+      split; first exact hlenL_eq.
+      split; first exact hlenL_ok.
+      split; first exact hlenL.
+      split; first by smt().
+      split; first by smt().
+      by smt().
+    by smt().
+  wp.
+  skip.
+  move=> &1 &2 /=.
+  move=> [ho hguards].
+  move: ho => [hrepr ho].
+  move: ho => [hbd ho].
+  move: ho => [hzetasp ho].
+  move: ho => [hzetas ho].
+  move: ho => [hzc_eq ho].
+  move: ho => [hlen_eq ho].
+  move: ho => [hlenok hzbase].
+  move: hguards => [hlen_pos hlen_guard].
+  split.
+  + split; first exact hrepr.
+    split.
+    + move=> i hi.
+      rewrite fwd_middle_start_const /const_bound.
+      exact (hbd i hi).
+    split; first exact hzetasp.
+    split; first exact hzetas.
+    split; first exact hzc_eq.
+    split; first exact hlen_eq.
+    split; first exact hlenok.
+    split; first exact hlen_pos.
+    by smt().
+  move=> rpL startL zcL rR startR zcR hnotL hnotR hm.
+  move: hm => [hreprL hm].
+  move: hm => [hbdL hm].
+  move: hm => [hzetaspL hm].
+  move: hm => [hzetasL hm].
+  move: hm => [hzcL hm].
+  move: hm => [hlenL_eq hm].
+  move: hm => [hlenL_ok hm].
+  move: hm => [hlenL_pos hm].
+  move: hm => [hstart_eqL hm].
+  move: hm => [hstart_rngL hstart_zcL].
+  have hstart_end : startL = 256 by smt().
+  have hshift : len{1} `|>>` 1 = len{1} %/ 2.
+  + by apply int_shr1_div2; smt().
+  have hlen_next :=
+    fwd_len_next_ok len{1} hlenL_ok hlenL_pos.
+  have hzbase_next :=
+    fwd_stage_zbase_exit len{1} zcL
+      hlenL_ok hlenL_pos _.
+  + by smt().
+  have hbdconst :
+    barray256_bound_by rpL
+      (const_bound
+        (fwd_stage_bound17 (len{1} `|>>` 1))).
+  + move=> i hi.
+    have htmp := hbdL i hi.
+    move: htmp.
+    rewrite hstart_end.
+    rewrite (fwd_middle_exit_const
+               (fwd_stage_bound17 len{1}) 256 i _ _).
+    + by move: hi; rewrite mem_range.
+    + trivial.
+    rewrite /const_bound /fwd_stage_bound17.
+    have hstage_next :=
+      fwd_stage_bound17_next len{1} hlenL_ok hlenL_pos.
+    smt().
+  split.
+  + split; first exact hreprL.
+    split; first exact hbdconst.
+    split; first exact hzetaspL.
+    split; first exact hzetasL.
+    split; first exact hzcL.
+    split; first by smt().
+    split; first by rewrite hshift; exact hlen_next.
+    by rewrite hshift; exact hzbase_next.
+  by rewrite hshift; smt().
+wp.
+skip.
+move=> &1 &2 /=.
+move=> [hpre hzetas2].
+split.
++ split.
+  + exact (NTT_Fq.poly_repr_bound_repr rp{1} r{2} 17 hpre).
+  split.
+  + rewrite /fwd_stage_bound17 /fwd_stage_bound.
+    exact (barray256_bound_by_const rp{1} 17
+             (NTT_Fq.poly_repr_bound_bound rp{1} r{2} 17 hpre)).
+  split; first by [].
+  split; first by rewrite /fwd_len_ok.
+  by rewrite /fwd_zbase.
+by smt().
+qed.
+
+lemma loop_poly_ntt_correct17 p :
+  hoare [Hpoly_loop.M._poly_ntt :
+    NTT_Fq.poly_repr_bound rp p 17 ==>
+    NTT_Fq.poly_repr_bound res (NTTFullSpec.full_ntt p) 25].
+proof.
+by conseq poly_ntt_core_ref17
+  (NTTFullAlgebra.ntt_full_ntt p) => /#.
+qed.
+
+lemma target_poly_ntt_correct17 p :
+  hoare [Target._poly_ntt :
+    NTT_Fq.poly_repr_bound rp p 17 ==>
+    NTT_Fq.poly_repr_bound res (NTTFullSpec.full_ntt p) 25].
+proof.
+have hloop_core :
+  hoare [Hpoly_loop.M._poly_ntt :
+    NTT_Fq.poly_repr_bound rp p 17 ==>
+    NTT_Fq.poly_repr_bound res (NTTFullSpec.full_ntt p) 25].
++ exact (loop_poly_ntt_correct17 p).
+by conseq TargetNTTRefinement.poly_ntt_loop_equiv hloop_core => /#.
+qed.
+
+lemma wide_polyvec_ntt_verify_unpack_count2_bound25
+    (xp0 : BArray8192.t) (p0 p1 : Rq.poly) :
+  hoare [Wide._polyvec_ntt :
+    xp = xp0 /\
+    count = W64.of_int verify_unpack_ntt_polys /\
+    verify_unpack_ntt_input_repr_bound17 xp0 p0 p1
+    ==>
+    verify_unpack_ntt_repr_bound25 res p0 p1 /\
+    KeygenM23MatrixSpec.word_tail_frame
+      xp0 res verify_unpack_ntt_words].
+proof.
+proc.
+rcondt 3; first by auto.
+rcondt 8; first by auto; call (_ : true); auto.
+rcondf 13; first by
+  auto; call (_ : true); auto; call (_ : true); auto.
+wp.
+call (target_poly_ntt_correct17 p1).
+wp.
+call (target_poly_ntt_correct17 p0).
+wp.
+skip.
+move=> &hr [-> [hcount hin]].
+move: hin.
+rewrite /verify_unpack_ntt_input_repr_bound17.
+move=> [hin0 hin1].
+have hbound0 :
+    0 <= 0 /\
+    0 + KeygenM23MatrixSpec.poly_words_i <=
+      KeygenM23MatrixSpec.array_words_i by
+  rewrite /KeygenM23MatrixSpec.poly_words_i
+          /KeygenM23MatrixSpec.array_words_i
+          /BArray8192.size /=.
+have hbound1 :
+    0 <= KeygenM23MatrixSpec.poly_words_i /\
+    KeygenM23MatrixSpec.poly_words_i +
+      KeygenM23MatrixSpec.poly_words_i <=
+      KeygenM23MatrixSpec.array_words_i by
+  rewrite /KeygenM23MatrixSpec.poly_words_i
+          /KeygenM23MatrixSpec.array_words_i
+          /BArray8192.size /=.
+have hrepr0 :
+    NTT_Fq.poly_repr_bound
+      (TargetKeygenM23WideSupport.poly_slice xp0 0) p0 17.
++ have hbridge :
+      (KeygenM23ArithmeticSpec.wide_slice_repr_bound xp0 0 p0 17 <=>
+       NTT_Fq.poly_repr_bound
+         (TargetKeygenM23WideSupport.poly_slice xp0 0) p0 17).
+  + apply TargetKeygenM23WideSupport.wide_slice_poly_repr_bound.
+    exact hbound0.
+  move: hin0.
+  by rewrite hbridge.
+have hrepr1 :
+    NTT_Fq.poly_repr_bound
+      (TargetKeygenM23WideSupport.poly_slice
+         xp0 KeygenM23MatrixSpec.poly_words_i) p1 17.
++ have hbridge :
+      (KeygenM23ArithmeticSpec.wide_slice_repr_bound
+         xp0 KeygenM23MatrixSpec.poly_words_i p1 17 <=>
+       NTT_Fq.poly_repr_bound
+         (TargetKeygenM23WideSupport.poly_slice
+            xp0 KeygenM23MatrixSpec.poly_words_i) p1 17).
+  + apply TargetKeygenM23WideSupport.wide_slice_poly_repr_bound.
+    exact hbound1.
+  move: hin1.
+  by rewrite hbridge.
+split.
++ exact hrepr0.
+move=> _ r0 hr0.
+have hslice1 :
+    TargetKeygenM23WideSupport.poly_slice
+      (TargetKeygenM23WideSupport.put_poly_slice xp0 0 r0)
+      KeygenM23MatrixSpec.poly_words_i =
+    TargetKeygenM23WideSupport.poly_slice
+      xp0 KeygenM23MatrixSpec.poly_words_i.
++ apply TargetKeygenM23WideSupport.poly_slice_put_other.
+  + exact hbound0.
+  + exact hbound1.
+  + right.
+    smt().
+split.
++ rewrite hslice1.
+  exact hrepr1.
+move=> _ r1 hr1.
+have hsame0 :
+    TargetKeygenM23WideSupport.poly_slice
+      (TargetKeygenM23WideSupport.put_poly_slice xp0 0 r0) 0 = r0.
++ apply TargetKeygenM23WideSupport.poly_slice_put_same.
+  exact hbound0.
+have hother10 :
+    TargetKeygenM23WideSupport.poly_slice
+      (TargetKeygenM23WideSupport.put_poly_slice
+        (TargetKeygenM23WideSupport.put_poly_slice xp0 0 r0)
+        KeygenM23MatrixSpec.poly_words_i r1) 0 =
+    TargetKeygenM23WideSupport.poly_slice
+      (TargetKeygenM23WideSupport.put_poly_slice xp0 0 r0) 0.
++ apply TargetKeygenM23WideSupport.poly_slice_put_other.
+  + exact hbound1.
+  + exact hbound0.
+  + left.
+    smt().
+have hsame1 :
+    TargetKeygenM23WideSupport.poly_slice
+      (TargetKeygenM23WideSupport.put_poly_slice
+        (TargetKeygenM23WideSupport.put_poly_slice xp0 0 r0)
+        KeygenM23MatrixSpec.poly_words_i r1)
+      KeygenM23MatrixSpec.poly_words_i = r1.
++ apply TargetKeygenM23WideSupport.poly_slice_put_same.
+  exact hbound1.
+have hpost0 :
+    KeygenM23ArithmeticSpec.wide_slice_repr_bound
+      (TargetKeygenM23WideSupport.put_poly_slice
+        (TargetKeygenM23WideSupport.put_poly_slice xp0 0 r0)
+        KeygenM23MatrixSpec.poly_words_i r1)
+      0 (NTTFullSpec.full_ntt p0) 25.
++ rewrite TargetKeygenM23WideSupport.wide_slice_poly_repr_bound 1:hbound0.
+  by rewrite hother10 hsame0.
+have hpost1 :
+    KeygenM23ArithmeticSpec.wide_slice_repr_bound
+      (TargetKeygenM23WideSupport.put_poly_slice
+        (TargetKeygenM23WideSupport.put_poly_slice xp0 0 r0)
+        KeygenM23MatrixSpec.poly_words_i r1)
+      KeygenM23MatrixSpec.poly_words_i
+      (NTTFullSpec.full_ntt p1) 25.
++ rewrite TargetKeygenM23WideSupport.wide_slice_poly_repr_bound 1:hbound1.
+  by rewrite hsame1.
+have htail0 :
+    KeygenM23MatrixSpec.word_tail_frame
+      xp0 xp0 verify_unpack_ntt_words by
+  rewrite /KeygenM23MatrixSpec.word_tail_frame.
+have htail1 :
+    KeygenM23MatrixSpec.word_tail_frame
+      xp0
+      (TargetKeygenM23WideSupport.put_poly_slice xp0 0 r0)
+      verify_unpack_ntt_words by
+  apply
+    (TargetKeygenM23WideSupport.word_tail_frame_put_before
+      xp0 xp0 0 verify_unpack_ntt_words r0);
+    [ rewrite /verify_unpack_ntt_words
+              /verify_unpack_ntt_polys
+              /KeygenM23MatrixSpec.poly_words_i /=
+    | rewrite /verify_unpack_ntt_words
+              /verify_unpack_ntt_polys
+              /KeygenM23MatrixSpec.poly_words_i
+              /KeygenM23MatrixSpec.array_words_i
+              /BArray8192.size /=
+    | exact htail0 ].
+have htail2 :
+    KeygenM23MatrixSpec.word_tail_frame
+      xp0
+      (TargetKeygenM23WideSupport.put_poly_slice
+        (TargetKeygenM23WideSupport.put_poly_slice xp0 0 r0)
+        KeygenM23MatrixSpec.poly_words_i r1)
+      verify_unpack_ntt_words by
+  apply
+    (TargetKeygenM23WideSupport.word_tail_frame_put_before
+      xp0 (TargetKeygenM23WideSupport.put_poly_slice xp0 0 r0)
+      KeygenM23MatrixSpec.poly_words_i verify_unpack_ntt_words r1);
+    [ rewrite /verify_unpack_ntt_words
+              /verify_unpack_ntt_polys
+              /KeygenM23MatrixSpec.poly_words_i /=
+    | rewrite /verify_unpack_ntt_words
+              /verify_unpack_ntt_polys
+              /KeygenM23MatrixSpec.poly_words_i
+              /KeygenM23MatrixSpec.array_words_i
+              /BArray8192.size /=
+    | exact htail1 ].
+simplify.
+rewrite /verify_unpack_ntt_repr_bound25.
+split.
++ split.
+  + exact hpost0.
+  + move: hpost1.
+    by rewrite /KeygenM23MatrixSpec.poly_words_i /=.
++ move: htail2.
+  by rewrite /verify_unpack_ntt_words
+             /verify_unpack_ntt_polys
+             /KeygenM23MatrixSpec.poly_words_i /=.
+qed.
+
+lemma verify_unpack_ntt_repr_bound25_forward_repr
+    (before after : BArray8192.t) (p0 p1 : Rq.poly) :
+  verify_unpack_ntt_input_repr_bound17 before p0 p1 =>
+  verify_unpack_ntt_repr_bound25 after p0 p1 =>
+  NTTRowProductSpec.vector_forward_repr
+    verify_unpack_ntt_polys
+    (fun col =>
+      KeygenM23ArithmeticSpec.wide_poly
+        after (col * KeygenM23MatrixSpec.poly_words_i))
+    (fun col =>
+      KeygenM23ArithmeticSpec.wide_poly
+        before (col * KeygenM23MatrixSpec.poly_words_i)).
+proof.
+rewrite /verify_unpack_ntt_input_repr_bound17
+        /verify_unpack_ntt_repr_bound25
+        /NTTRowProductSpec.vector_forward_repr.
+move=> [hin0 hin1] [hout0 hout1] col hcol.
+case (col = 0) => h0.
++ subst col.
+  move: hin0 hout0.
+  rewrite /KeygenM23ArithmeticSpec.wide_slice_repr_bound.
+  by move=> [-> _] [-> _].
+have h1 : col = 1 by smt().
+subst col.
+move: hin1 hout1.
+rewrite /KeygenM23ArithmeticSpec.wide_slice_repr_bound
+        /KeygenM23MatrixSpec.poly_words_i /=.
+by move=> [-> _] [-> _].
+qed.
+
+lemma parent_polyvec_ntt_verify_unpack_count2_bound25
+    (xp0 : BArray8192.t) (p0 p1 : Rq.poly) :
+  hoare [Parent._polyvec_ntt :
+    xp = xp0 /\
+    count = W64.of_int verify_unpack_ntt_polys /\
+    verify_unpack_ntt_input_repr_bound17 xp0 p0 p1
+    ==>
+    verify_unpack_ntt_repr_bound25 res p0 p1 /\
+    KeygenM23MatrixSpec.word_tail_frame
+      xp0 res verify_unpack_ntt_words].
+proof.
+have hwide := wide_polyvec_ntt_verify_unpack_count2_bound25 xp0 p0 p1.
+by conseq VerifyUnpackV3NttPostFreeze.parent_polyvec_ntt_equiv_wide_count2
+  hwide => /#.
+qed.
+
+lemma parent_polyvec_ntt_verify_unpack_count2_correct
+    (xp0 : BArray8192.t) (p0 p1 : Rq.poly) :
+  hoare [Parent._polyvec_ntt :
+    xp = xp0 /\
+    count = W64.of_int verify_unpack_ntt_polys /\
+    verify_unpack_ntt_input_repr_bound17 xp0 p0 p1
+    ==>
+    NTTRowProductSpec.vector_forward_repr
+      verify_unpack_ntt_polys
+      (fun col =>
+        KeygenM23ArithmeticSpec.wide_poly
+          res (col * KeygenM23MatrixSpec.poly_words_i))
+      (fun col =>
+        KeygenM23ArithmeticSpec.wide_poly
+          xp0 (col * KeygenM23MatrixSpec.poly_words_i)) /\
+    KeygenM23MatrixSpec.word_tail_frame
+      xp0 res verify_unpack_ntt_words].
+proof.
+have hparent := parent_polyvec_ntt_verify_unpack_count2_bound25 xp0 p0 p1.
+conseq hparent => //=.
+move=> &m [_ [_ hin]] result [hout htail].
+split.
++ exact
+    (verify_unpack_ntt_repr_bound25_forward_repr
+      xp0 result p0 p1 hin hout).
++ exact htail.
+qed.
+
+lemma verify_unpack_polyvec_ntt_count2_bound25
+    (xp0 : BArray8192.t) (p0 p1 : Rq.poly) :
+  hoare [Verify._polyvec_ntt :
+    xp = xp0 /\
+    count = W64.of_int verify_unpack_ntt_polys /\
+    verify_unpack_ntt_input_repr_bound17 xp0 p0 p1
+    ==>
+    verify_unpack_ntt_repr_bound25 res p0 p1 /\
+    KeygenM23MatrixSpec.word_tail_frame
+      xp0 res verify_unpack_ntt_words].
+proof.
+by conseq VerifyUnpackV3NttPostFreeze.verify_unpack_polyvec_ntt_equiv_parent
+  (parent_polyvec_ntt_verify_unpack_count2_bound25 xp0 p0 p1) => /#.
+qed.
+
+lemma verify_unpack_polyvec_ntt_count2_correct
+    (xp0 : BArray8192.t) (p0 p1 : Rq.poly) :
+  hoare [Verify._polyvec_ntt :
+    xp = xp0 /\
+    count = W64.of_int verify_unpack_ntt_polys /\
+    verify_unpack_ntt_input_repr_bound17 xp0 p0 p1
+    ==>
+    NTTRowProductSpec.vector_forward_repr
+      verify_unpack_ntt_polys
+      (fun col =>
+        KeygenM23ArithmeticSpec.wide_poly
+          res (col * KeygenM23MatrixSpec.poly_words_i))
+      (fun col =>
+        KeygenM23ArithmeticSpec.wide_poly
+          xp0 (col * KeygenM23MatrixSpec.poly_words_i)) /\
+    KeygenM23MatrixSpec.word_tail_frame
+      xp0 res verify_unpack_ntt_words].
+proof.
+by conseq VerifyUnpackV3NttPostFreeze.verify_unpack_polyvec_ntt_equiv_parent
+  (parent_polyvec_ntt_verify_unpack_count2_correct xp0 p0 p1) => /#.
+qed.
+
+lemma verify_unpack_polyvec_ntt_count2_full_correct
+    (xp0 : BArray8192.t) (p0 p1 : Rq.poly) :
+  hoare [Verify._polyvec_ntt :
+    xp = xp0 /\
+    count = W64.of_int verify_unpack_ntt_polys /\
+    verify_unpack_ntt_input_repr_bound17 xp0 p0 p1
+    ==>
+    verify_unpack_ntt_repr_bound25 res p0 p1 /\
+    NTTRowProductSpec.vector_forward_repr
+      verify_unpack_ntt_polys
+      (fun col =>
+        KeygenM23ArithmeticSpec.wide_poly
+          res (col * KeygenM23MatrixSpec.poly_words_i))
+      (fun col =>
+        KeygenM23ArithmeticSpec.wide_poly
+          xp0 (col * KeygenM23MatrixSpec.poly_words_i)) /\
+    KeygenM23MatrixSpec.word_tail_frame
+      xp0 res verify_unpack_ntt_words].
+proof.
+conseq
+  (verify_unpack_polyvec_ntt_count2_bound25 xp0 p0 p1)
+  (verify_unpack_polyvec_ntt_count2_correct xp0 p0 p1) => />.
+qed.
+
+lemma verify_unpack_polyvec_ntt_count2_full_correct17
+    (xp0 : BArray8192.t) (p0 p1 : Rq.poly) :
+  hoare [Verify._polyvec_ntt :
+    xp = xp0 /\
+    count = W64.of_int verify_unpack_ntt_polys /\
+    verify_unpack_ntt_input_repr_bound17 xp0 p0 p1
+    ==>
+    verify_unpack_ntt_repr_bound25 res p0 p1 /\
+    NTTRowProductSpec.vector_forward_repr
+      verify_unpack_ntt_polys
+      (fun col =>
+        KeygenM23ArithmeticSpec.wide_poly
+          res (col * KeygenM23MatrixSpec.poly_words_i))
+      (fun col =>
+        KeygenM23ArithmeticSpec.wide_poly
+          xp0 (col * KeygenM23MatrixSpec.poly_words_i)) /\
+    KeygenM23MatrixSpec.word_tail_frame
+      xp0 res verify_unpack_ntt_words].
+proof.
+exact (verify_unpack_polyvec_ntt_count2_full_correct xp0 p0 p1).
+qed.
+
+end VerifyUnpackV3NttBound17PostFreeze.
