haetae-topdown-easycrypt/post-freeze/VerifyUnpackV3PreNttBoundPostFreeze.ec
@@ -1,0 +1,132 @@
+require import AllCore IntDiv Ring.
+
+from Jasmin require import JModel_x86.
+
+import SLH64.
+
+require import BArray2752 BArray8192 BArray32768 Fq
+  KeygenM23ArithmeticSpec KeygenM23MatrixSpec
+  VerifyUnpackV3AssemblyPostFreeze VerifyUnpackV3PreNttPostFreeze
+  VerifyUnpackVkM23CoefficientsPostFreeze.
+
+import VerifyUnpackV3AssemblyPostFreeze.
+
+theory VerifyUnpackV3PreNttBoundPostFreeze.
+
+op pre_ntt_source_bound
+    (vkp : BArray2752.t) (mat : BArray32768.t) : bool =
+  forall i, 0 <= i < mode2_vec_words =>
+    W32.to_uint
+      (BArray32768.get32 mat (firstcol_slot_idx i)) < 64513 /\
+    W32.to_uint
+      (VerifyUnpackVkM23CoefficientsPostFreeze.unpack_vk_coeff_word vkp i)
+      < 32768.
+
+op pre_ntt_active_bound17 (a : BArray8192.t) : bool =
+  forall i, 0 <= i < mode2_vec_words =>
+    Fq.bw32 (BArray8192.get32 a i) 17.
+
+lemma mode2_pre_ntt_word_bound17 (a b : W32.t) :
+  0 <= W32.to_uint a < 64513 =>
+  0 <= W32.to_uint b < 32768 =>
+  Fq.bw32 (mode2_pre_ntt_word a b) 17.
+proof.
+move=> ha hb.
+have heq :
+    mode2_pre_ntt_word a b =
+    W32.of_int (2 * (W32.to_uint a - 2 * W32.to_uint b)).
++ rewrite /mode2_pre_ntt_word /(`<<`) !W8.of_uintK /=;
+  rewrite -(W32.to_uintK a) -(W32.to_uintK b).
+  rewrite !W32.shlMP 1:/#.
+  rewrite !W32.to_uintK_small 1:/# 1:/#.
+  rewrite W32.of_intS' W32.shlMP 1:/#.
+  congr; ring.
+rewrite heq /Fq.bw32 W32.to_sintK_small; smt().
+qed.
+
+lemma pre_ntt_active_bound17_of_prefix_frame
+    (vkp : BArray2752.t)
+    (mat0 mat : BArray32768.t) (after : BArray8192.t) :
+  pre_ntt_source_bound vkp mat0 =>
+  VerifyUnpackV3PreNttPostFreeze.pre_ntt_prefix
+    vkp mat after mode2_vec_words =>
+  mat_firstcol_frame mat0 mat =>
+  pre_ntt_active_bound17 after.
+proof.
+move=> hsource hprefix hframe.
+rewrite /pre_ntt_active_bound17 => i hi.
+rewrite /VerifyUnpackV3PreNttPostFreeze.pre_ntt_prefix in hprefix.
+rewrite hprefix 1:hi hframe 1:hi.
+apply mode2_pre_ntt_word_bound17.
++ have ha := W32.to_uint_cmp
+    (BArray32768.get32 mat0 (firstcol_slot_idx i)).
+  have hs := hsource i hi.
+  smt().
+have hb := W32.to_uint_cmp
+  (VerifyUnpackVkM23CoefficientsPostFreeze.unpack_vk_coeff_word vkp i).
+have hs := hsource i hi.
+smt().
+qed.
+
+lemma pre_ntt_active_bound17_repr_self (a : BArray8192.t) :
+  pre_ntt_active_bound17 a =>
+  KeygenM23ArithmeticSpec.wide_slice_repr_bound
+    a 0 (KeygenM23ArithmeticSpec.wide_poly a 0) 17 /\
+  KeygenM23ArithmeticSpec.wide_slice_repr_bound
+    a KeygenM23MatrixSpec.poly_words_i
+      (KeygenM23ArithmeticSpec.wide_poly
+        a KeygenM23MatrixSpec.poly_words_i) 17.
+proof.
+move=> hbound.
+split.
++ apply KeygenM23ArithmeticSpec.wide_slice_repr_bound_self.
+  rewrite /KeygenM23ArithmeticSpec.wide_slice_bound => j hj.
+  apply hbound.
+  rewrite /mode2_vec_words /mode2_rows /poly_words
+          /KeygenM23MatrixSpec.poly_words_i in hj.
+  rewrite /mode2_vec_words /mode2_rows /poly_words.
+  smt().
+apply KeygenM23ArithmeticSpec.wide_slice_repr_bound_self.
+rewrite /KeygenM23ArithmeticSpec.wide_slice_bound => j hj.
+apply hbound.
+rewrite /mode2_vec_words /mode2_rows /poly_words
+        /KeygenM23MatrixSpec.poly_words_i in hj.
+rewrite /mode2_vec_words /mode2_rows /poly_words
+        /KeygenM23MatrixSpec.poly_words_i.
+smt().
+qed.
+
+lemma actual_verify_unpack_post_expand_pre_ntt_mode2_bound17
+    (bp0 : BArray8192.t) (vkp0 : BArray2752.t)
+    (mat0 : BArray32768.t) :
+  hoare [
+    VerifyUnpackV3PreNttPostFreeze.ActualVerifyUnpackPostExpandPreNttMode2.run :
+    bp = bp0 /\ vkp = vkp0 /\ matp = mat0 /\
+    pre_ntt_source_bound vkp0 mat0
+    ==>
+    VerifyUnpackV3PreNttPostFreeze.pre_ntt_prefix
+      vkp0 res.`2 res.`1 mode2_vec_words /\
+    mat_firstcol_frame mat0 res.`2 /\
+    pre_ntt_active_bound17 res.`1 /\
+    KeygenM23ArithmeticSpec.wide_slice_repr_bound
+      res.`1 0 (KeygenM23ArithmeticSpec.wide_poly res.`1 0) 17 /\
+    KeygenM23ArithmeticSpec.wide_slice_repr_bound
+      res.`1 KeygenM23MatrixSpec.poly_words_i
+        (KeygenM23ArithmeticSpec.wide_poly
+          res.`1 KeygenM23MatrixSpec.poly_words_i) 17].
+proof.
+conseq
+  (VerifyUnpackV3PreNttPostFreeze.actual_verify_unpack_post_expand_pre_ntt_mode2_word_exact
+     bp0 vkp0 mat0).
++ auto.
+move=> &m hpre result [hprefix hframe].
+have hsource : pre_ntt_source_bound vkp0 mat0 by
+  move: hpre => />.
+have hbound :=
+  pre_ntt_active_bound17_of_prefix_frame
+    vkp0 mat0 result.`2 result.`1 hsource hprefix hframe.
+have hrepr := pre_ntt_active_bound17_repr_self result.`1 hbound.
+by auto.
+qed.
+
+end VerifyUnpackV3PreNttBoundPostFreeze.
